WIP: orrectness of compilation of for

compiler/core/Imp/Lang/ImpEJsonRewrite.v
@@ -26,6 +26,7 @@ Require Import JsAst.JsNumber.
 Require Import EJsonRuntime.
 Require Import Imp.
 Require Import ImpEJson.
+Require Import ImpEJsonVars.
 Require Import ImpEJsonEval.
 
 Section ImpEJsonRewrite.
@@ -34,22 +35,29 @@ Section ImpEJsonRewrite.
   Context {fejson:foreign_ejson}.
   Context {fejruntime:foreign_ejson_runtime}.
 
+  Lemma imp_ejson_stmt_eval_env_simpl h stmt l1 x v l2:
+    ~ In x (domain l2) ->
+    imp_ejson_stmt_eval h stmt (l1 ++ (x, v) :: l2) = imp_ejson_stmt_eval h stmt (l1 ++ l2).
+  Proof.
+    admit.
+  Admitted.
+
   Section ForRewrite.
+
     (* Rewriting functional for into imperative for loop is now isolated *)
-    Fixpoint imp_ejson_stmt_for_rewrite (avoid: list string) (stmt: imp_ejson_stmt): imp_ejson_stmt :=
+    Fixpoint imp_ejson_stmt_for_rewrite (stmt: imp_ejson_stmt): imp_ejson_stmt :=
       match stmt with
       | ImpStmtBlock lv ls =>
         ImpStmtBlock
           lv
-          (map (imp_ejson_stmt_for_rewrite ((List.map fst lv) ++ avoid)) ls)
+          (map imp_ejson_stmt_for_rewrite ls)
       | ImpStmtAssign v e =>
         ImpStmtAssign v e
       | ImpStmtFor v e s =>
-        let avoid := v :: avoid in
-        let src_id := fresh_var "src" avoid in
-        let avoid := src_id :: avoid in
+        let avoid := v :: imp_ejson_stmt_free_vars stmt in
         let i_id := fresh_var "i" avoid in
         let avoid := i_id :: avoid in
+        let src_id := fresh_var "src" avoid in
         let src := ImpExprVar src_id in
         let i := ImpExprVar i_id in
         ImpStmtBlock
@@ -62,26 +70,497 @@ Section ImpEJsonRewrite.
                                   [ ImpExprOp EJsonOpArrayLength [ src ] ; ImpExprConst (ejbigint 1) ])
               (ImpStmtBlock
                  [ (v, Some (ImpExprOp EJsonOpArrayAccess [ src; i ])) ]
-                 [ imp_ejson_stmt_for_rewrite avoid s ]) ]
+                 [ imp_ejson_stmt_for_rewrite s ]) ]
       | ImpStmtForRange v e1 e2 s =>
-        ImpStmtForRange v
-                        e1
-                        e2
-                        (imp_ejson_stmt_for_rewrite (v :: avoid) s)
+        ImpStmtForRange v e1 e2
+                        (imp_ejson_stmt_for_rewrite s)
       | ImpStmtIf e s1 s2 =>
         ImpStmtIf e
-                  (imp_ejson_stmt_for_rewrite avoid s1)
-                  (imp_ejson_stmt_for_rewrite avoid s2)
+                  (imp_ejson_stmt_for_rewrite s1)
+                  (imp_ejson_stmt_for_rewrite s2)
       end.
+
   End ForRewrite.
 
   Section CorrectnessForRewrite.
-    Lemma imp_ejson_stmt_for_rewrite_correct h (σ : pd_jbindings) (stmt:imp_ejson_stmt) :
-      forall avoid,
-        imp_ejson_stmt_eval h stmt σ =
-        imp_ejson_stmt_eval h (imp_ejson_stmt_for_rewrite avoid stmt)  σ.
+
+    Lemma number_iterations A (l: list A):
+      (ImpEval.nb_iter 0 (BinInt.Z.sub (BinInt.Z.of_nat (List.length l)) 1)) = length l.
+    Proof.
+      unfold ImpEval.nb_iter; simpl.
+      induction (Datatypes.length l); [ simpl; reflexivity | ].
+      rewrite BinInt.Z.sub_1_r.
+      rewrite Znat.Nat2Z.inj_succ.
+      rewrite <- BinInt.Zpred_succ.
+      case n; [ simpl; reflexivity | ].
+      intros.
+      rewrite <- BinInt.Zminus_0_l_reverse.
+      rewrite Znat.Nat2Z.id.
+      simpl; reflexivity.
+    Qed.
+
+    Fixpoint list_n_nat {A} (n:nat) (l:list A) :=
+      match n with
+      | 0 => nil
+      | S n' =>
+        match l with
+        | nil => nil
+        | x :: l' => x :: (list_n_nat n' l')
+        end
+      end.
+
+    Fixpoint list_tail_n_nat {A} n (l: list A) :=
+    List.rev (list_n_nat n (List.rev l)).
+
+    Lemma for_corr_aux
+      (l_init : list ejson)
+      (j: nat)
+      (v : var)
+      (e : imp_expr)
+      (stmt : imp_stmt)
+      (h : BrandRelation.brand_relation_t)
+      (l : list ejson)
+      (σ : pd_jbindings) :
+      let i := fresh_var "i"
+                         (v :: imp_ejson_expr_free_vars e ++
+                            remove string_eqdec v (imp_ejson_stmt_free_vars stmt))
+      in
+      let src := fresh_var "src"
+                           (i :: v :: imp_ejson_expr_free_vars e ++
+                              remove string_eqdec v (imp_ejson_stmt_free_vars stmt))
+      in
+      (lookup string_eqdec σ src = Some (Some (ejarray l_init))) ->
+      (list_tail_n_nat (List.length l) l_init = l) ->
+      (j + Datatypes.length l = List.length l_init) ->
+      (fix for_fun (dl : list imp_ejson_model) (σ₁ : list (var * option imp_ejson_model)) {struct dl} :
+         option (list (var * option imp_ejson_model)) :=
+         match dl with
+         | [] => Some σ₁
+         | d :: dl' =>
+           match imp_ejson_stmt_eval h stmt ((v, Some d) :: σ₁) with
+           | Some (_ :: σ₂) => for_fun dl' σ₂
+           | _ => None
+           end
+         end) l σ =
+       match
+         (fix for_range (n : nat) (n1 : BinNums.Z) (σ₁ : list (var * option imp_ejson_model)) {struct n} :
+            option (list (var * option imp_ejson_model)) :=
+            match n with
+            | 0 => Some σ₁
+            | S n' =>
+                match
+                  match
+                    match
+                      match
+                        olift (imp_ejson_op_eval EJsonOpArrayAccess)
+                          match
+                            olift (fun x : option imp_ejson_model => x)
+                              ((fix
+                                lookup (l0 : list (string * option imp_ejson_model)) (a : string) {struct l0} :
+                                  option (option imp_ejson_model) :=
+                                  match l0 with
+                                  | [] => None
+                                  | (f', v') :: os => if EquivDec.equiv_dec a f' then Some v' else lookup os a
+                                  end) σ₁
+                                 src)
+                          with
+                          | Some x' => Some [x'; imp_ejson_Z_to_data n1]
+                          | None => None
+                          end
+                      with
+                      | Some d =>
+                          Some
+                            ((v, Some d)
+                             :: (i, Some (imp_ejson_Z_to_data n1))
+                             :: σ₁)
+                      | None => None
+                      end
+                    with
+                    | Some x' => imp_ejson_stmt_eval h stmt x'
+                    | None => None
+                    end
+                  with
+                  | Some (_ :: σ') => Some σ'
+                  | _ => None
+                  end
+                with
+                | Some (_ :: σ₂) => for_range n' (BinInt.Z.add n1 1) σ₂
+                | _ => None
+                end
+            end) (j + Datatypes.length l) (BinInt.Z_of_nat j)
+           ((src, Some (ejarray l)) :: σ)
+       with
+       | Some (_ :: σ') => Some σ'
+       | _ => None
+       end.
+    Proof.
+    Qed.
+
+
+
+
+
+    (* Lemma for_range_ind h src i j n s σ : *)
+    (*   let for_range_stmt := ImpStmtForRange i j n s in *)
+    (*   j <= n -> *)
+    (*   imp_ejson_expr_eval h (ImpExprVar src) σ = Some l_init -> *)
+      
+
+
+    Lemma for_corr v e stmt :
+      forall h σ,
+      let for_stmt := ImpStmtFor v e stmt in
+      let for_range_stmt :=
+        let avoid := v :: imp_ejson_stmt_free_vars (ImpStmtFor v e stmt) in
+        let i_id := fresh_var "i" avoid in
+        let avoid := i_id :: avoid in
+        let src_id := fresh_var "src" avoid in
+        let src := ImpExprVar src_id in
+        let i := ImpExprVar i_id in
+        ImpStmtBlock
+          [ (src_id, Some e) ]
+          [ ImpStmtForRange
+              i_id
+              (ImpExprConst (ejbigint 0))
+              (* XXX Use src.length - 1, consistent with semantic of 'for i1 to i2 do ... done' loop *)
+              (ImpExprRuntimeCall EJsonRuntimeNatMinus
+                                  [ ImpExprOp EJsonOpArrayLength [ src ] ; ImpExprConst (ejbigint 1) ])
+              (ImpStmtBlock
+                 [ (v, Some (ImpExprOp EJsonOpArrayAccess [ src; i ])) ]
+                 [ stmt ]) ]
+      in
+      imp_ejson_stmt_eval h for_stmt σ =
+      imp_ejson_stmt_eval h for_range_stmt σ.
+    Proof.
+      simpl.
+      intros.
+      unfold ImpEval.imp_decls_eval.
+      unfold olift.
+      simpl.
+      match_destr.
+      unfold lookup.
+      case (EquivDec.equiv_dec
+              (fresh_var "src"
+                 (fresh_var "i"
+                    (v
+                     :: ImpVars.imp_expr_free_vars e ++
+                        remove string_eqdec v (imp_ejson_stmt_free_vars stmt))
+                  :: v
+                     :: ImpVars.imp_expr_free_vars e ++
+                        remove string_eqdec v (imp_ejson_stmt_free_vars stmt)))
+              (fresh_var "src"
+                 (fresh_var "i"
+                    (v
+                     :: ImpVars.imp_expr_free_vars e ++
+                        remove string_eqdec v (imp_ejson_stmt_free_vars stmt))
+                  :: v
+                     :: ImpVars.imp_expr_free_vars e ++
+                        remove string_eqdec v (imp_ejson_stmt_free_vars stmt))));
+        [ intro Eq; clear Eq | congruence ].
+      case (EquivDec.equiv_dec
+               (fresh_var "i"
+                  (v
+                   :: ImpVars.imp_expr_free_vars e ++
+                      remove string_eqdec v (imp_ejson_stmt_free_vars stmt)))
+               (fresh_var "i"
+                  (v
+                   :: ImpVars.imp_expr_free_vars e ++
+                      remove string_eqdec v (imp_ejson_stmt_free_vars stmt))));
+        try congruence; intro Eq; clear Eq.
+      unfold imp_ejson_model_to_list.
+      case i; simpl; try reflexivity.
+      intros l.
+      rewrite number_iterations.
+      generalize σ; clear σ.
+
+
+      induction l; [ simpl; reflexivity | ].
+      intros.
+      simpl.
+
+        unfold olift.
+        case (EquivDec.equiv_dec
+                (fresh_var "src"
+                   (fresh_var "i"
+                      (v
+                       :: ImpVars.imp_expr_free_vars e ++
+                          remove string_eqdec v (imp_ejson_stmt_free_vars stmt))
+                    :: v
+                       :: ImpVars.imp_expr_free_vars e ++
+                          remove string_eqdec v (imp_ejson_stmt_free_vars stmt)))
+                (fresh_var "src"
+                   (fresh_var "i"
+                      (v
+                       :: ImpVars.imp_expr_free_vars e ++
+                          remove string_eqdec v (imp_ejson_stmt_free_vars stmt))
+                    :: v
+                       :: ImpVars.imp_expr_free_vars e ++
+                          remove string_eqdec v (imp_ejson_stmt_free_vars stmt))));
+          [ intro Eq; clear Eq | congruence].
+        simpl.
+        rewrite (imp_ejson_stmt_eval_env_simpl _ _
+                   ((v, Some a)
+                    :: (fresh_var "i"
+                          (v
+                           :: ImpVars.imp_expr_free_vars e ++ remove string_eqdec v (imp_ejson_stmt_free_vars stmt)),
+                       Some (imp_ejson_Z_to_data 0)) :: [])
+                   (fresh_var "src"
+                     (fresh_var "i"
+                        (v
+                         :: ImpVars.imp_expr_free_vars e ++
+                            remove string_eqdec v (imp_ejson_stmt_free_vars stmt))
+                      :: v
+                         :: ImpVars.imp_expr_free_vars e ++
+                            remove string_eqdec v (imp_ejson_stmt_free_vars stmt)))
+                   (Some (ejarray (a :: l)))
+                   σ);
+          [ | admit ].
+        rewrite (imp_ejson_stmt_eval_env_simpl _ _
+                   ((v, Some a) :: [])
+                   (fresh_var "i"
+                     (v :: ImpVars.imp_expr_free_vars e ++ remove string_eqdec v (imp_ejson_stmt_free_vars stmt)))
+                   (Some (imp_ejson_Z_to_data 0))
+                   σ);
+          [ | admit ].
+        simpl.
+        unfold var.
+        unfold imp_ejson_model.
+        case (@imp_ejson_stmt_eval fejson fejruntime h stmt
+                (@cons (prod string (option (@ejson fejson)))
+                   (@pair string (option (@ejson fejson)) v (@Some (@ejson fejson) a)) σ));
+          [ | simpl; reflexivity].
+        intros σ'.
+        clear i a σ.
+        match_destr.
+        rewrite IHl; clear IHl.
+        unfold olift.
+        simpl.
+
+
+    Qed.
+
+
+    Lemma for_body h src i v n n' a stmt σ1:
+      (* match *)
+      (*   ImpEval.imp_decls_eval *)
+      (*     ((fresh_var "i" *)
+      (*         (fresh_var "src" *)
+      (*            ((ImpVars.imp_expr_free_vars e ++ *)
+      (*              remove string_eqdec v (imp_ejson_stmt_free_vars stmt)) ++ *)
+      (*             v :: imp_ejson_stmt_bound_vars stmt) *)
+      (*          :: (ImpVars.imp_expr_free_vars e ++ *)
+      (*              remove string_eqdec v (imp_ejson_stmt_free_vars stmt)) ++ *)
+      (*             v :: imp_ejson_stmt_bound_vars stmt), Some (imp_ejson_Z_to_data n1)) *)
+      (*      :: σ₁) *)
+      (*     [(v, *)
+      (*      Some *)
+      (*        (ImpExprOp EJsonOpArrayAccess *)
+      (*           [ImpExprVar *)
+      (*              (fresh_var "src" *)
+      (*                 ((ImpVars.imp_expr_free_vars e ++ *)
+      (*                   remove string_eqdec v (imp_ejson_stmt_free_vars stmt)) ++ *)
+      (*                  v :: imp_ejson_stmt_bound_vars stmt)); *)
+      (*           ImpExprVar *)
+      (*             (fresh_var "i" *)
+      (*                (fresh_var "src" *)
+      (*                   ((ImpVars.imp_expr_free_vars e ++ *)
+      (*                     remove string_eqdec v (imp_ejson_stmt_free_vars stmt)) ++ *)
+      (*                    v :: imp_ejson_stmt_bound_vars stmt) *)
+      (*                 :: (ImpVars.imp_expr_free_vars e ++ *)
+      (*                     remove string_eqdec v (imp_ejson_stmt_free_vars stmt)) ++ *)
+      (*                    v :: imp_ejson_stmt_bound_vars stmt))]))] *)
+      (* with *)
+      (* | Some x'0 => imp_ejson_stmt_eval h (imp_ejson_stmt_for_rewrite stmt) x'0 *)
+      (* | None => None *)
+      (* end *)
+      imp_ejson_decls_eval h
+        ((i, Some (imp_ejson_Z_to_data n)) :: σ1)
+        [(v, Some (ImpExprOp EJsonOpArrayAccess [ImpExprVar src; ImpExprVar i]))]
+      =
+      Some ((v, a) :: (i, n') :: σ1)
+      ->
+      match
+        imp_ejson_decls_eval h
+          ((i, Some (imp_ejson_Z_to_data n)) :: σ1)
+          [(v, Some (ImpExprOp EJsonOpArrayAccess [ImpExprVar src; ImpExprVar i]))]
+      with
+      | Some σ2 => imp_ejson_stmt_eval h (imp_ejson_stmt_for_rewrite stmt) σ2
+      | None => None
+      end
+      =
+      imp_ejson_stmt_eval h stmt ((v, a) :: (i, n') :: σ1).
     Proof.
       admit.
+    Admitted.
+
+    Lemma imp_ejson_stmt_for_rewrite_correct h (σ : pd_jbindings) (stmt:imp_ejson_stmt) :
+        imp_ejson_stmt_eval h stmt σ =
+        imp_ejson_stmt_eval h (imp_ejson_stmt_for_rewrite stmt)  σ.
+    Proof.
+      generalize σ.
+      imp_stmt_cases (induction stmt) Case; intros; simpl.
+      - Case "ImpStmtBlock"%string.
+        unfold ImpEval.imp_decls_erase.
+        assert ((map imp_ejson_stmt_for_rewrite sl) = sl) as Heq;
+          [ | rewrite Heq; reflexivity].
+        induction sl; trivial.
+        simpl.
+        inversion H.
+        rewrite (IHsl H3).
+        admit.
+      - Case "ImpStmtAssign"%string.
+        reflexivity.
+      - Case "ImpStmtFor"%string.
+        unfold ImpEval.imp_decls_eval.
+        unfold olift.
+        simpl.
+        match_destr.
+        unfold lookup.
+        (* case (EquivDec.equiv_dec (fresh_var "src" (v :: avoid)) (fresh_var "src" (v :: avoid))); *)
+        (*   try congruence; intro Eq; clear Eq. *)
+Set Printing Depth 100.
+        case (EquivDec.equiv_dec
+                (fresh_var "src"
+                   (fresh_var "i"
+                      (v
+                       :: ImpVars.imp_expr_free_vars e ++
+                          remove string_eqdec v (imp_ejson_stmt_free_vars stmt))
+                    :: v
+                       :: ImpVars.imp_expr_free_vars e ++
+                          remove string_eqdec v (imp_ejson_stmt_free_vars stmt)))
+                (fresh_var "src"
+                   (fresh_var "i"
+                      (v
+                       :: ImpVars.imp_expr_free_vars e ++
+                          remove string_eqdec v (imp_ejson_stmt_free_vars stmt))
+                    :: v
+                       :: ImpVars.imp_expr_free_vars e ++
+                          remove string_eqdec v (imp_ejson_stmt_free_vars stmt))));
+          [ intro Eq; clear Eq | congruence ].
+        case (EquivDec.equiv_dec
+                 (fresh_var "i"
+                    (v
+                     :: ImpVars.imp_expr_free_vars e ++
+                        remove string_eqdec v (imp_ejson_stmt_free_vars stmt)))
+                 (fresh_var "i"
+                    (v
+                     :: ImpVars.imp_expr_free_vars e ++
+                        remove string_eqdec v (imp_ejson_stmt_free_vars stmt))));
+          try congruence; intro Eq; clear Eq.
+        unfold imp_ejson_model_to_list.
+        case i; simpl; try reflexivity.
+        intros l.
+        rewrite number_iterations.
+        generalize σ0; clear σ0.
+        induction l; [ simpl; reflexivity | ].
+        intros.
+        simpl.
+        unfold olift.
+        case (EquivDec.equiv_dec
+                (fresh_var "src"
+                   (fresh_var "i"
+                      (v
+                       :: ImpVars.imp_expr_free_vars e ++
+                          remove string_eqdec v (imp_ejson_stmt_free_vars stmt))
+                    :: v
+                       :: ImpVars.imp_expr_free_vars e ++
+                          remove string_eqdec v (imp_ejson_stmt_free_vars stmt)))
+                (fresh_var "src"
+                   (fresh_var "i"
+                      (v
+                       :: ImpVars.imp_expr_free_vars e ++
+                          remove string_eqdec v (imp_ejson_stmt_free_vars stmt))
+                    :: v
+                       :: ImpVars.imp_expr_free_vars e ++
+                          remove string_eqdec v (imp_ejson_stmt_free_vars stmt))));
+          [ intro Eq; clear Eq | congruence].
+        simpl.
+        rewrite <- (IHstmt ((@cons (prod string (option (@imp_ejson_model fejson)))
+               (@pair string (option (@imp_ejson_model fejson)) v (@Some (@imp_ejson_model fejson) a))
+               (@cons (prod var (option (@imp_ejson_model fejson)))
+                  (@pair var (option (@imp_ejson_model fejson))
+                     (fresh_var
+                        (String (Ascii.Ascii true false false true false true true false) EmptyString)
+                        (@cons var v
+                           (@app var
+                              (@ImpVars.imp_expr_free_vars (@imp_ejson_model fejson) imp_ejson_op
+                                 (@imp_ejson_runtime_op fejson fejruntime) e)
+                              (@remove string string_eqdec v
+                                 (@imp_ejson_stmt_free_vars fejson fejruntime stmt)))))
+                     (@Some (@imp_ejson_model fejson) (@imp_ejson_Z_to_data fejson BinNums.Z0)))
+                  (@cons (prod string (option (@imp_ejson_model fejson)))
+                     (@pair string (option (@imp_ejson_model fejson))
+                        (fresh_var
+                           (String (Ascii.Ascii true true false false true true true false)
+                              (String (Ascii.Ascii false true false false true true true false)
+                                 (String (Ascii.Ascii true true false false false true true false)
+                                    EmptyString)))
+                           (@cons string
+                              (fresh_var
+                                 (String (Ascii.Ascii true false false true false true true false)
+                                    EmptyString)
+                                 (@cons var v
+                                    (@app var
+                                       (@ImpVars.imp_expr_free_vars (@imp_ejson_model fejson) imp_ejson_op
+                                          (@imp_ejson_runtime_op fejson fejruntime) e)
+                                       (@remove string string_eqdec v
+                                          (@imp_ejson_stmt_free_vars fejson fejruntime stmt)))))
+                              (@cons var v
+                                 (@app var
+                                    (@ImpVars.imp_expr_free_vars (@imp_ejson_model fejson) imp_ejson_op
+                                       (@imp_ejson_runtime_op fejson fejruntime) e)
+                                    (@remove string string_eqdec v
+                                       (@imp_ejson_stmt_free_vars fejson fejruntime stmt))))))
+                        (@Some (@imp_ejson_model fejson) (@ejarray fejson (@cons (@ejson fejson) a l))))
+                     σ0))))).
+        rewrite (imp_ejson_stmt_eval_env_simpl _ _
+                   ((v, Some a)
+                    :: (fresh_var "i"
+                          (v
+                           :: ImpVars.imp_expr_free_vars e ++ remove string_eqdec v (imp_ejson_stmt_free_vars stmt)),
+                       Some (imp_ejson_Z_to_data 0)) :: [])
+                   (fresh_var "src"
+                     (fresh_var "i"
+                        (v
+                         :: ImpVars.imp_expr_free_vars e ++
+                            remove string_eqdec v (imp_ejson_stmt_free_vars stmt))
+                      :: v
+                         :: ImpVars.imp_expr_free_vars e ++
+                            remove string_eqdec v (imp_ejson_stmt_free_vars stmt)))
+                   (Some (ejarray (a :: l)))
+                   σ0);
+          [ | admit ].
+        rewrite (imp_ejson_stmt_eval_env_simpl _ _
+                   ((v, Some a) :: [])
+                   (fresh_var "i"
+                     (v :: ImpVars.imp_expr_free_vars e ++ remove string_eqdec v (imp_ejson_stmt_free_vars stmt)))
+                   (Some (imp_ejson_Z_to_data 0))
+                   σ0);
+          [ | admit ].
+        simpl.
+        unfold var.
+        unfold imp_ejson_model.
+        case (imp_ejson_stmt_eval h stmt ((v, Some a) :: σ0)); [ | simpl; reflexivity].
+        intros σ'.
+        clear i a σ0 σ.
+        match_destr.
+        rewrite IHl; clear IHl.
+        unfold olift.
+        simpl.
+        admit.
+      - Case "ImpStmtForRange"%string.
+        repeat match_destr.
+        generalize (ImpEval.nb_iter z z0).
+        intros.
+        clear z0.
+        generalize z σ0.
+        induction n; intros; try reflexivity.
+        rewrite <- IHstmt.
+        repeat match_destr.
+      - Case "ImpStmtIf"%string.
+        rewrite <- (IHstmt1 σ0).
+        rewrite <- (IHstmt2 σ0).
+        reflexivity.
     Admitted.
   End CorrectnessForRewrite.
 
